theories/Factor_Scope_Admission.thy
@@ -1,0 +1,669 @@
+theory Factor_Scope_Admission
+  imports Factor_Positive_Admission Factor_Scope_Forwarding Factor_Native_Syntax_Determination
+begin
+
+section \<open>The complete forwarding profile has ordinary finite admission\<close>
+
+abbreviation scope_forwarding_argument ::
+  "factor_term \<Rightarrow> factor_term \<Rightarrow> factor_term \<Rightarrow> factor_term \<Rightarrow>
+    factor_term \<Rightarrow> factor_term \<Rightarrow> factor_term \<Rightarrow> factor_term" where
+  "scope_forwarding_argument e u r k x y z \<equiv>
+    citation_observation_argument e u r (Pair_Term k (source_root_argument x y z))"
+
+abbreviation scope_forwarding_pattern ::
+  "'a term_pattern \<Rightarrow> 'a term_pattern \<Rightarrow> 'a term_pattern \<Rightarrow> 'a term_pattern \<Rightarrow>
+    'a term_pattern \<Rightarrow> 'a term_pattern \<Rightarrow> 'a term_pattern \<Rightarrow> 'a term_pattern" where
+  "scope_forwarding_pattern e u r k x y z \<equiv>
+    citation_observation_pattern e u r (Pattern_Pair k (source_root_pattern x y z))"
+
+abbreviation scope_forwarding_result :: "factor_term \<Rightarrow> bool" where
+  "scope_forwarding_result t \<equiv> \<exists>E e u r k x y z.
+    t=scope_forwarding_argument e (use_data_term u) (Payload_Term r) (definition_site_value k) x y z \<and>
+    environment_value_presents E e \<and> native_scope_forwarding_at E u r k x y z"
+
+definition scope_forwarding_schema :: "(nat,nat,nat) factor_schema" where
+  "scope_forwarding_schema=data_rule
+    (scope_forwarding_pattern data_x data_y data_z data_w (Pattern_Variable 4) (Pattern_Variable 5) (Pattern_Variable 6))
+    {(0,72,citation_observation_pattern data_x data_y data_z (Pattern_Payload [])),
+     (1,37,artifact_lookup_pattern data_x data_y (Pattern_Variable 7)),
+     (2,34,Pattern_Pair (Pattern_Pair (Pattern_Variable 7) data_z)
+       (data_list_pattern [Pattern_Pair (Pattern_Variable 8) (Pattern_Variable 10),
+         Pattern_Pair (Pattern_Variable 9) (Pattern_Variable 11)])),
+     (3,32,Pattern_Pair (Pattern_Pair (Pattern_Variable 7) (Pattern_Variable 11))
+       (data_list_pattern [Pattern_Pair (Pattern_Variable 12) (Pattern_Variable 13)])),
+     (4,56,scoped_instantiation_pattern data_x data_y (Pattern_Variable 10)
+       (data_list_pattern [Pattern_Pair (Pattern_Variable 14) (Pattern_Variable 14)])
+       (Pattern_Variable 14) (Pattern_Variable 17) (Pattern_Variable 18)),
+     (5,56,scoped_instantiation_pattern data_x data_y (Pattern_Variable 10)
+       (data_list_pattern [Pattern_Pair (Pattern_Variable 14) (Pattern_Target (Whole_Artifact empty_artifact))])
+       (Pattern_Target (Whole_Artifact empty_artifact)) (Pattern_Variable 17) (Pattern_Variable 18)),
+     (6,65,schema_instantiation_pattern data_x data_y (Pattern_Variable 13)
+       (data_list_pattern [Pattern_Pair (Pattern_Variable 15) (Pattern_Variable 15)])
+       (Pattern_Variable 15)
+       (data_list_pattern [Pattern_Pair (Pattern_Variable 16) (Pattern_Pair data_w
+         (package_subject_pattern (Pattern_Variable 4) (Pattern_Variable 5) (Pattern_Variable 6) (Pattern_Variable 15)))])
+       (Pattern_Payload [])),
+     (7,65,schema_instantiation_pattern data_x data_y (Pattern_Variable 13)
+       (data_list_pattern [Pattern_Pair (Pattern_Variable 15) (Pattern_Target (Whole_Artifact empty_artifact))])
+       (Pattern_Target (Whole_Artifact empty_artifact))
+       (data_list_pattern [Pattern_Pair (Pattern_Variable 16) (Pattern_Pair data_w
+         (package_subject_pattern (Pattern_Variable 4) (Pattern_Variable 5) (Pattern_Variable 6)
+           (Pattern_Target (Whole_Artifact empty_artifact))))])
+       (Pattern_Payload []))}"
+
+definition scope_forwarding_system :: "(nat,nat,nat,nat) schema_system" where
+  "scope_forwarding_system=add_view_definition native_positive_admission_system 116 data_x {(0,scope_forwarding_schema)}"
+
+lemma scope_forwarding_system_formed [simp]: "schema_system_formed scope_forwarding_system"
+  unfolding scope_forwarding_system_def
+  by (rule add_recursive_definition_formed[OF native_positive_admission_system_formed])
+    (auto simp: scope_forwarding_schema_def
+      schema_formed_def schema_dependencies_def single_valued_def rel_dom_def rel_ran_def octets_formed_def)
+
+lemma scope_forwarding_definitions [simp]:
+  "system_definitions scope_forwarding_system=insert 116 (system_definitions native_positive_admission_system)"
+  by (simp add: scope_forwarding_system_def)
+
+lemma scope_forwarding_call:
+  "schema_call_formed scope_forwarding_system d t \<longleftrightarrow>
+    d\<in>system_definitions scope_forwarding_system \<and> term_formed t"
+  using added_variable_calls[OF native_positive_admission_system_formed
+    scope_forwarding_system_formed[unfolded scope_forwarding_system_def] native_positive_admission_call]
+  by (simp only: scope_forwarding_system_def[symmetric])
+
+lemma scope_forwarding_old_meaning:
+  assumes "d\<in>system_definitions native_positive_admission_system"
+  shows "(d,t)\<in>positive_meaning scope_forwarding_system \<longleftrightarrow>
+    (d,t)\<in>positive_meaning native_positive_admission_system"
+  using added_definition_preserves_old(2)[OF native_positive_admission_system_formed
+    scope_forwarding_system_formed[unfolded scope_forwarding_system_def], of d t] assms
+  by (auto simp: scope_forwarding_system_def)
+
+lemma scope_forwarding_clause [simp]:
+  "((116,c),S)\<in>system_clauses scope_forwarding_system \<longleftrightarrow> (c,S)\<in>{(0,scope_forwarding_schema)}"
+proof -
+  have owned: "((d,c),S)\<in>system_clauses native_positive_admission_system \<Longrightarrow>
+    d\<in>system_definitions native_positive_admission_system" for d c S
+    using native_positive_admission_system_formed unfolding schema_system_formed_def by blast
+  have absent: "((116,c),S)\<notin>system_clauses native_positive_admission_system" by (auto dest: owned)
+  show ?thesis using absent by (simp add: scope_forwarding_system_def)
+qed
+
+lemma scope_forwarding_definition_meaning:
+  assumes "d\<in>system_definitions definition_call_admission_system"
+  shows "(d,t)\<in>positive_meaning scope_forwarding_system \<longleftrightarrow>
+    (d,t)\<in>positive_meaning definition_call_admission_system"
+  using assms
+  by (simp add: scope_forwarding_old_meaning native_positive_admission_old_meaning
+    positive_query_old_meaning environment_inclusion_old_meaning artifact_inclusion_old_meaning
+    replay_admission_old_meaning retention_admission_slot_meaning replay_slot_reading_old_meaning
+    replay_source_reading_graph_meaning proof_graph_membership_node_meaning
+    proof_node_reading_base_meaning admitted_instantiation_previous_meaning
+    package_admission_previous_meaning package_closure_previous_meaning)
+
+lemma scope_forwarding_components:
+  "(72,t)\<in>positive_meaning scope_forwarding_system \<longleftrightarrow>
+    (72,t)\<in>positive_meaning definition_call_admission_system"
+  "(37,t)\<in>positive_meaning scope_forwarding_system \<longleftrightarrow>
+    (37,t)\<in>positive_meaning artifact_lookup_system"
+  "(34,t)\<in>positive_meaning scope_forwarding_system \<longleftrightarrow>
+    (34,t)\<in>positive_meaning record_admission_system"
+  "(32,t)\<in>positive_meaning scope_forwarding_system \<longleftrightarrow>
+    (32,t)\<in>positive_meaning family_admission_system"
+  "(56,t)\<in>positive_meaning scope_forwarding_system \<longleftrightarrow>
+    (56,t)\<in>positive_meaning scoped_instantiation_system"
+  "(65,t)\<in>positive_meaning scope_forwarding_system \<longleftrightarrow>
+    (65,t)\<in>positive_meaning schema_instantiation_system"
+  using scope_forwarding_definition_meaning[of 72 t] scope_forwarding_definition_meaning[of 37 t]
+    scope_forwarding_definition_meaning[of 34 t] scope_forwarding_definition_meaning[of 32 t]
+    scope_forwarding_definition_meaning[of 56 t] scope_forwarding_definition_meaning[of 65 t]
+    definition_call_admission_components(1-3)[of t]
+    definition_call_admission_old_meaning[of 32 t] schema_family_admission_components(2)[of t]
+    definition_call_admission_instantiation_meaning[of 65 t] by auto
+
+lemma scope_forwarding_valuation:
+  "(116,t)\<in>positive_meaning scope_forwarding_system \<longleftrightarrow>
+    (\<exists>h::nat\<Rightarrow>factor_term. (\<forall>j\<in>{0,1,2,3,4,5,6,7,8,9,10,11,12,13,14,15,16,17,18}. term_formed (h j)) \<and>
+      t=scope_forwarding_argument (h 0) (h 1) (h 2) (h 3) (h 4) (h 5) (h 6) \<and>
+      (72,citation_observation_argument (h 0) (h 1) (h 2) (Payload_Term []))\<in>positive_meaning definition_call_admission_system \<and>
+      (37,artifact_lookup_argument (h 0) (h 1) (h 7))\<in>positive_meaning artifact_lookup_system \<and>
+      (34,rooted_rows_argument (h 7) (h 2) (pair_list_term [(h 8,h 10),(h 9,h 11)]))
+        \<in>positive_meaning record_admission_system \<and>
+      (32,rooted_rows_argument (h 7) (h 11) (pair_list_term [(h 12,h 13)]))
+        \<in>positive_meaning family_admission_system \<and>
+      (56,scoped_instantiation_argument (h 0) (h 1) (h 10)
+        (pair_list_term [(h 14,h 14)]) (h 14) (h 17) (h 18))\<in>positive_meaning scoped_instantiation_system \<and>
+      (56,scoped_instantiation_argument (h 0) (h 1) (h 10)
+        (pair_list_term [(h 14,Target_Term (Whole_Artifact empty_artifact))])
+        (Target_Term (Whole_Artifact empty_artifact)) (h 17) (h 18))\<in>positive_meaning scoped_instantiation_system \<and>
+      (65,schema_instantiation_argument (h 0) (h 1) (h 13) (pair_list_term [(h 15,h 15)]) (h 15)
+        (pair_list_term [(h 16,Pair_Term (h 3) (package_subject_argument (h 4) (h 5) (h 6) (h 15)))])
+        (Payload_Term []))\<in>positive_meaning schema_instantiation_system \<and>
+      (65,schema_instantiation_argument (h 0) (h 1) (h 13)
+        (pair_list_term [(h 15,Target_Term (Whole_Artifact empty_artifact))])
+        (Target_Term (Whole_Artifact empty_artifact))
+        (pair_list_term [(h 16,Pair_Term (h 3) (package_subject_argument (h 4) (h 5) (h 6)
+          (Target_Term (Whole_Artifact empty_artifact))))])
+        (Payload_Term []))\<in>positive_meaning schema_instantiation_system)"
+proof -
+  have family: "((116,c),S)\<in>system_clauses scope_forwarding_system \<longleftrightarrow>
+      c=0 \<and> S=scope_forwarding_schema" for c S by simp
+  have ordinary: "schema_material_premises scope_forwarding_schema={}"
+    by (simp add: scope_forwarding_schema_def)
+  have boundary: "schema_call_formed scope_forwarding_system 116
+    (evaluate_pattern h (schema_conclusion scope_forwarding_schema))"
+    if assignment: "\<forall>a\<in>schema_variables scope_forwarding_schema. term_formed (h a)" for h
+    using assignment by (auto simp: scope_forwarding_call scope_forwarding_schema_def schema_variables_def)
+  have variables: "schema_variables scope_forwarding_schema={0,1,2,3,4,5,6,7,8,9,10,11,12,13,14,15,16,17,18}"
+    by (auto simp: scope_forwarding_schema_def schema_variables_def)
+  have head: "evaluate_pattern h (schema_conclusion scope_forwarding_schema)=
+    scope_forwarding_argument (h 0) (h 1) (h 2) (h 3) (h 4) (h 5) (h 6)" for h
+    by (simp add: scope_forwarding_schema_def)
+  have calls: "(\<forall>s d p. (s,d,p)\<in>schema_premises scope_forwarding_schema \<longrightarrow>
+      (d,evaluate_pattern h p)\<in>positive_meaning scope_forwarding_system) \<longleftrightarrow>
+      (72,citation_observation_argument (h 0) (h 1) (h 2) (Payload_Term []))\<in>positive_meaning definition_call_admission_system \<and>
+      (37,artifact_lookup_argument (h 0) (h 1) (h 7))\<in>positive_meaning artifact_lookup_system \<and>
+      (34,rooted_rows_argument (h 7) (h 2) (pair_list_term [(h 8,h 10),(h 9,h 11)]))
+        \<in>positive_meaning record_admission_system \<and>
+      (32,rooted_rows_argument (h 7) (h 11) (pair_list_term [(h 12,h 13)]))
+        \<in>positive_meaning family_admission_system \<and>
+      (56,scoped_instantiation_argument (h 0) (h 1) (h 10)
+        (pair_list_term [(h 14,h 14)]) (h 14) (h 17) (h 18))\<in>positive_meaning scoped_instantiation_system \<and>
+      (56,scoped_instantiation_argument (h 0) (h 1) (h 10)
+        (pair_list_term [(h 14,Target_Term (Whole_Artifact empty_artifact))])
+        (Target_Term (Whole_Artifact empty_artifact)) (h 17) (h 18))\<in>positive_meaning scoped_instantiation_system \<and>
+      (65,schema_instantiation_argument (h 0) (h 1) (h 13) (pair_list_term [(h 15,h 15)]) (h 15)
+        (pair_list_term [(h 16,Pair_Term (h 3) (package_subject_argument (h 4) (h 5) (h 6) (h 15)))])
+        (Payload_Term []))\<in>positive_meaning schema_instantiation_system \<and>
+      (65,schema_instantiation_argument (h 0) (h 1) (h 13)
+        (pair_list_term [(h 15,Target_Term (Whole_Artifact empty_artifact))])
+        (Target_Term (Whole_Artifact empty_artifact))
+        (pair_list_term [(h 16,Pair_Term (h 3) (package_subject_argument (h 4) (h 5) (h 6)
+          (Target_Term (Whole_Artifact empty_artifact))))])
+        (Payload_Term []))\<in>positive_meaning schema_instantiation_system" for h
+  proof -
+    have rows: "(\<forall>s d p. (s,d,p)\<in>schema_premises scope_forwarding_schema \<longrightarrow>
+        (d,evaluate_pattern h p)\<in>positive_meaning scope_forwarding_system) \<longleftrightarrow>
+      (\<forall>(s,d,p)\<in>schema_premises scope_forwarding_schema.
+        (d,evaluate_pattern h p)\<in>positive_meaning scope_forwarding_system)"
+      by (auto split: prod.splits)
+    show ?thesis by (simp only: rows)
+      (simp add: scope_forwarding_schema_def scope_forwarding_components)
+  qed
+  note equation=ordinary_single_clause_valuation[OF family ordinary boundary, where t=t]
+  show ?thesis by (rule equation[unfolded variables head calls])
+qed
+
+section \<open>Finite row shapes expose their actual coordinates\<close>
+
+lemma binding_rows_singleton_iff:
+  "binding_rows_term xs=pair_list_term [(a,t)] \<longleftrightarrow> (\<exists>b. a=Payload_Term b \<and> xs=[(b,t)])"
+  by (simp only: pair_list_term_injective; cases xs) (auto split: prod.splits)
+
+lemma call_rows_singleton_iff:
+  "call_instance_rows_term xs=pair_list_term [(s,Pair_Term k t)] \<longleftrightarrow>
+    (\<exists>a d. s=Payload_Term a \<and> k=definition_site_value d \<and> xs=[(a,d,t)])"
+  by (simp only: pair_list_term_injective; cases xs)
+    (auto simp: call_instance_value_def split: prod.splits)
+
+lemma native_definition_record_interface:
+  assumes raw: "native_definition_at E u r p C" and source: "artifact_at E u R"
+    and rec: "record_at R r ps [i,m]"
+  shows "\<exists>I K. scoped_pattern_at E u i p I K"
+proof -
+  obtain A qs j n I K where parts: "environment_formed E" "artifact_at E u A"
+    "record_at A r qs [j,n]" "scoped_pattern_at E u j p I K"
+    using raw by (auto simp: native_definition_at_def)
+  have same: "A=R" by (rule environment_artifact_unique[OF parts(1,2) source])
+  have other: "record_at R r qs [j,n]" using parts(3) same by simp
+  have "j=i" using record_at_unique[OF other rec] by auto
+  then show ?thesis using parts(4) by blast
+qed
+
+
+lemma scoped_variable_readings:
+  assumes source: "environment_value_presents E e" and address: "octets_formed a"
+    and orders: "distinct Is" "distinct Ks"
+  shows "scoped_pattern_at E u r (Pattern_Variable a) (set Is) (set Ks) \<longleftrightarrow>
+    (56,scoped_instantiation_argument e (use_data_term u) (Payload_Term r)
+      (binding_rows_term [(a,Payload_Term a)]) (Payload_Term a)
+      (data_list_term (map Payload_Term Is)) (data_list_term (map Payload_Term Ks)))
+        \<in>positive_meaning scoped_instantiation_system \<and>
+    (56,scoped_instantiation_argument e (use_data_term u) (Payload_Term r)
+      (binding_rows_term [(a,Target_Term (Whole_Artifact empty_artifact))])
+      (Target_Term (Whole_Artifact empty_artifact))
+      (data_list_term (map Payload_Term Is)) (data_list_term (map Payload_Term Ks)))
+        \<in>positive_meaning scoped_instantiation_system"
+  using scoped_pattern_two_instances[OF source, where p="Pattern_Variable a" and u=u and r=r
+    and xs="[(a,Payload_Term a)]" and ys="[(a,Target_Term (Whole_Artifact empty_artifact))]"
+    and Is=Is and Ks=Ks] address orders by auto
+
+lemma scope_schema_readings:
+  assumes source: "environment_value_presents E e" and address: "octets_formed b"
+    and fields: "term_formed x" "term_formed y" "term_formed z"
+  shows "native_schema_at E u r (scope_call_schema b s k x y z) \<longleftrightarrow>
+    (65,schema_instantiation_argument e (use_data_term u) (Payload_Term r)
+      (binding_rows_term [(b,Payload_Term b)]) (Payload_Term b)
+      (call_instance_rows_term [(s,k,package_subject_argument x y z (Payload_Term b))])
+      (binding_rows_term []))\<in>positive_meaning schema_instantiation_system \<and>
+    (65,schema_instantiation_argument e (use_data_term u) (Payload_Term r)
+      (binding_rows_term [(b,Target_Term (Whole_Artifact empty_artifact))])
+      (Target_Term (Whole_Artifact empty_artifact))
+      (call_instance_rows_term [(s,k,package_subject_argument x y z (Target_Term (Whole_Artifact empty_artifact)))])
+      (binding_rows_term []))\<in>positive_meaning schema_instantiation_system"
+proof -
+  have first: "schema_instance (scope_call_schema b s k x y z) {(b,Payload_Term b)}
+      (Payload_Term b) {(s,k,package_subject_argument x y z (Payload_Term b))}"
+    by (rule scope_call_schema_instance[OF fields]) (use address in simp)
+  have second: "schema_instance (scope_call_schema b s k x y z) {(b,Target_Term (Whole_Artifact empty_artifact))}
+      (Target_Term (Whole_Artifact empty_artifact))
+      {(s,k,package_subject_argument x y z (Target_Term (Whole_Artifact empty_artifact)))}"
+    by (rule scope_call_schema_instance[OF fields]) simp
+  show ?thesis by (rule native_schema_two_instances[OF source, where B="{b}"])
+    (use first second in \<open>auto simp: material_instance_relation_def scope_call_schema_def\<close>)
+qed
+
+section \<open>Soundness recovers the whole definition, not a selected execution\<close>
+
+theorem scope_forwarding_sound:
+  assumes holds: "(116,t)\<in>positive_meaning scope_forwarding_system"
+  shows "scope_forwarding_result t"
+proof -
+  obtain h :: "nat\<Rightarrow>factor_term" where
+    formed: "\<forall>j\<in>{0,1,2,3,4,5,6,7,8,9,10,11,12,13,14,15,16,17,18}. term_formed (h j)"
+    and shape: "t=scope_forwarding_argument (h 0) (h 1) (h 2) (h 3) (h 4) (h 5) (h 6)"
+    and reads:
+      "(72,citation_observation_argument (h 0) (h 1) (h 2) (Payload_Term []))\<in>positive_meaning definition_call_admission_system"
+      "(37,artifact_lookup_argument (h 0) (h 1) (h 7))\<in>positive_meaning artifact_lookup_system"
+      "(34,rooted_rows_argument (h 7) (h 2) (pair_list_term [(h 8,h 10),(h 9,h 11)]))
+        \<in>positive_meaning record_admission_system"
+      "(32,rooted_rows_argument (h 7) (h 11) (pair_list_term [(h 12,h 13)]))
+        \<in>positive_meaning family_admission_system"
+      "(56,scoped_instantiation_argument (h 0) (h 1) (h 10)
+        (pair_list_term [(h 14,h 14)]) (h 14) (h 17) (h 18))\<in>positive_meaning scoped_instantiation_system"
+      "(56,scoped_instantiation_argument (h 0) (h 1) (h 10)
+        (pair_list_term [(h 14,Target_Term (Whole_Artifact empty_artifact))])
+        (Target_Term (Whole_Artifact empty_artifact)) (h 17) (h 18))\<in>positive_meaning scoped_instantiation_system"
+      "(65,schema_instantiation_argument (h 0) (h 1) (h 13) (pair_list_term [(h 15,h 15)]) (h 15)
+        (pair_list_term [(h 16,Pair_Term (h 3) (package_subject_argument (h 4) (h 5) (h 6) (h 15)))])
+        (Payload_Term []))\<in>positive_meaning schema_instantiation_system"
+      "(65,schema_instantiation_argument (h 0) (h 1) (h 13)
+        (pair_list_term [(h 15,Target_Term (Whole_Artifact empty_artifact))])
+        (Target_Term (Whole_Artifact empty_artifact))
+        (pair_list_term [(h 16,Pair_Term (h 3) (package_subject_argument (h 4) (h 5) (h 6)
+          (Target_Term (Whole_Artifact empty_artifact))))])
+        (Payload_Term []))\<in>positive_meaning schema_instantiation_system"
+    using holds by (simp only: scope_forwarding_valuation) blast
+  obtain E u R where source: "environment_value_presents E (h 0)" "h 1=use_data_term u"
+    "artifact_at E u R" "artifact_value_presents R (h 7)"
+    using reads(2) by (simp only: artifact_lookup_exact factor_term.inject) blast
+  obtain r p q i m where rec: "h 2=Payload_Term r" "h 8=Payload_Term p" "h 10=Payload_Term i"
+    "h 9=Payload_Term q" "h 11=Payload_Term m" "record_at R r [p,q] [i,m]"
+    using reads(3) by (simp only: list.map prod.case record_admission_pair_fields[OF source(4)]) blast
+  obtain pat C where raw: "native_definition_at E u r pat C"
+    using reads(1) by (simp only: source(2) rec(1) definition_call_admission_on_values[OF source(1)]) blast
+  obtain xs where family: "pair_list_term [(h 12,h 13)]=data_list_term (map address_pair_data xs)"
+    "family_at R m (set xs)"
+    using reads(4) by (simp only: rec(5) family_admission_at_source[OF source(4)] factor_term.inject) blast
+  have rows: "[Pair_Term (h 12) (h 13)]=map address_pair_data xs"
+    using family(1) by (simp only: list.map prod.case data_list_term_injective)
+  obtain c a where row: "h 12=Payload_Term c" "h 13=Payload_Term a" "xs=[(c,a)]"
+    using rows by (cases xs) (auto simp: address_pair_data_def split: prod.splits)
+  have singleton: "family_at R m {(c,a)}" using family(2) row(3) by simp
+  obtain bs Is Ks where interface_rows:
+    "pair_list_term [(h 14,h 14)]=binding_rows_term bs"
+    "h 17=data_list_term (map Payload_Term Is)" "h 18=data_list_term (map Payload_Term Ks)"
+    "distinct Is" "distinct Ks"
+    using reads(5) by (simp only: source(2) rec(3) scoped_instantiation_at_source[OF source(1)]
+      factor_term.inject inj_eq[OF use_data_term_injective]) blast
+  obtain ib where ib: "h 14=Payload_Term ib"
+    using interface_rows(1)[symmetric] by (simp only: binding_rows_singleton_iff) blast
+  have ib_formed: "octets_formed ib" using formed ib by auto
+  have interface: "scoped_pattern_at E u i (Pattern_Variable ib) (set Is) (set Ks)"
+    using reads(5,6)[unfolded source(2) rec(3) ib interface_rows(2,3)]
+    by (simp only: scoped_variable_readings[OF source(1) ib_formed interface_rows(4,5)]) simp
+  obtain bs qs where schema_rows:
+    "pair_list_term [(h 15,h 15)]=binding_rows_term bs"
+    "pair_list_term [(h 16,Pair_Term (h 3) (package_subject_argument (h 4) (h 5) (h 6) (h 15)))]=call_instance_rows_term qs"
+    using reads(7) by (simp only: source(2) row(2) schema_instantiation_at_source[OF source(1)]
+      factor_term.inject inj_eq[OF use_data_term_injective]) blast
+  obtain b where b: "h 15=Payload_Term b"
+    using schema_rows(1)[symmetric] by (simp only: binding_rows_singleton_iff) blast
+  obtain s k where call: "h 16=Payload_Term s" "h 3=definition_site_value k"
+    using schema_rows(2)[symmetric] by (simp only: call_rows_singleton_iff) blast
+  have b_formed: "octets_formed b" using formed b by auto
+  have fields: "term_formed (h 4)" "term_formed (h 5)" "term_formed (h 6)" using formed by auto
+  let ?S="scope_call_schema b s k (h 4) (h 5) (h 6)"
+  have schema: "native_schema_at E u a ?S"
+    using reads(7,8)[unfolded source(2) row(2) b call]
+    by (simp only: scope_schema_readings[OF source(1) b_formed fields])
+      (simp add: call_instance_value_def)
+  obtain I K where other_interface: "scoped_pattern_at E u i pat I K"
+    using native_definition_record_interface[OF raw source(3) rec(6)] by blast
+  have pat: "pat=Pattern_Variable ib" using scoped_pattern_unique[OF other_interface interface] by blast
+  have family_read: "native_schema_family_at E u m C"
+    by (rule native_definition_record_family[OF raw source(3) rec(6)])
+  have same_schema: "native_schema_at E u a T \<longleftrightarrow> T=?S" for T
+  proof
+    assume other: "native_schema_at E u a T"
+    show "T=?S" by (rule native_schema_unique[OF other schema])
+  next
+    assume "T=?S"
+    then show "native_schema_at E u a T" using schema by simp
+  qed
+  have clauses: "(d,T)\<in>C \<longleftrightarrow> d=c \<and> T=?S" for d T
+    by (simp only: native_schema_family_at_graph(1)[OF family_read source(3) singleton])
+      (simp add: same_schema)
+  have C: "C={(c,?S)}"
+  proof (rule set_eqI)
+    fix q :: "local_address \<times> local_address option native_schema"
+    obtain d T where shape: "q=(d,T)" by (cases q)
+    show "q\<in>C \<longleftrightarrow> q\<in>{(c,?S)}" by (simp only: shape clauses; simp)
+  qed
+  have forwarding: "native_scope_forwarding_at E u r k (h 4) (h 5) (h 6)"
+    using raw pat C by (auto simp: native_scope_forwarding_at_def)
+  show ?thesis by (rule exI[of _ E], rule exI[of _ "h 0"], rule exI[of _ u],
+      rule exI[of _ r], rule exI[of _ k], rule exI[of _ "h 4"],
+      rule exI[of _ "h 5"], rule exI[of _ "h 6"])
+    (use shape source(1,2) rec(1) call(2) forwarding in simp)
+qed
+
+
+lemma scoped_pattern_variables_formed:
+  assumes raw: "scoped_pattern_at E u r p I K"
+  shows "\<forall>a\<in>pattern_variables p. octets_formed a"
+proof -
+  obtain R b where parts: "environment_formed E" "artifact_at E u R"
+    "binder_scope_at R b (pattern_variables p)"
+    using raw by (auto simp: scoped_pattern_at_def)
+  have formed: "exact_formed R" using parts(1,2) by (auto simp: environment_formed_def)
+  show ?thesis using binder_scope_properties(2)[OF parts(3)] formed
+    by (auto simp: exact_formed_def)
+qed
+
+section \<open>Every actual forwarding definition supplies the finite readings\<close>
+
+theorem scope_forwarding_complete:
+  assumes source: "environment_value_presents E e"
+    and forwarding: "native_scope_forwarding_at E u r k x y z"
+  shows "(116,scope_forwarding_argument e (use_data_term u) (Payload_Term r) (definition_site_value k) x y z)
+    \<in>positive_meaning scope_forwarding_system"
+proof -
+  obtain ib c b s where raw: "native_definition_at E u r (Pattern_Variable ib)
+      {(c,scope_call_schema b s k x y z)}"
+    using forwarding by (auto simp: native_scope_forwarding_at_def)
+  let ?S="scope_call_schema b s k x y z"
+  obtain R ps i m I K where parts: "artifact_at E u R" "record_at R r ps [i,m]"
+    "scoped_pattern_at E u i (Pattern_Variable ib) I K"
+    "native_schema_family_at E u m {(c,?S)}"
+    using raw by (auto simp: native_definition_at_def)
+  obtain A M a where origin: "artifact_at E u A" "family_at A m M" "(c,a)\<in>M" "native_schema_at E u a ?S"
+    using native_schema_family_origin[OF parts(4), of c ?S] by auto
+  have ef: "environment_formed E" using environment_value_presents_formed[OF source] by blast
+  have same: "A=R" by (rule environment_artifact_unique[OF ef origin(1) parts(1)])
+  have family: "family_at R m M" using origin(2) same by simp
+  have socket: "d=c" if row: "(d,w)\<in>M" for d w
+  proof -
+    obtain T where member: "(d,T)\<in>{(c,?S)}"
+      using native_schema_family_at_graph(2)[OF parts(4) parts(1) family, rule_format, OF row] by blast
+    show "d=c" using member by simp
+  qed
+  have keys: "rel_dom M={c}"
+  proof (rule set_eqI, rule iffI)
+    fix d assume "d\<in>rel_dom M"
+    then obtain w where row: "(d,w)\<in>M" by (auto simp: rel_dom_def)
+    have "d=c" by (rule socket[OF row])
+    then show "d\<in>{c}" by simp
+  next
+    fix d assume "d\<in>{c}"
+    then have "d=c" by simp
+    then show "d\<in>rel_dom M" using rel_domI[OF origin(3)] by simp
+  qed
+  have sv: "single_valued M" using family by (simp add: family_at_def)
+  have M: "M={(c,a)}"
+  proof
+    show "M\<subseteq>{(c,a)}"
+    proof
+      fix q assume member: "q\<in>M"
+      obtain d w where shape: "q=(d,w)" by (cases q)
+      have row: "(d,w)\<in>M" using member shape by simp
+      have key: "d=c" using rel_domI[OF row] keys by simp
+      have same_output: "w=a" using single_valued_outputs[OF sv row] origin(3) key by blast
+      show "q\<in>{(c,a)}" using shape key same_output by simp
+    qed
+    show "{(c,a)}\<subseteq>M" using origin(3) by simp
+  qed
+  have singleton: "family_at R m {(c,a)}" using family M by simp
+  have fields: "term_formed x" "term_formed y" "term_formed z"
+    by (rule native_scope_forwarding_fields[OF forwarding])+
+  have ib_formed: "octets_formed ib" using scoped_pattern_variables_formed[OF parts(3)] by simp
+  have b_formed: "octets_formed b" using native_schema_variables_formed[OF origin(4)] by simp
+  obtain Is where Is: "set Is=I" "distinct Is"
+    using scoped_pattern_formed[OF parts(3)] finite_distinct_list[of I] by blast
+  obtain Ks where Ks: "set Ks=K" "distinct Ks"
+    using scoped_pattern_formed[OF parts(3)] finite_distinct_list[of K] by blast
+  have interface: "scoped_pattern_at E u i (Pattern_Variable ib) (set Is) (set Ks)"
+    using parts(3) Is(1) Ks(1) by simp
+  have interface_reads:
+    "(56,scoped_instantiation_argument e (use_data_term u) (Payload_Term i)
+      (binding_rows_term [(ib,Payload_Term ib)]) (Payload_Term ib)
+      (data_list_term (map Payload_Term Is)) (data_list_term (map Payload_Term Ks)))
+        \<in>positive_meaning scoped_instantiation_system"
+    "(56,scoped_instantiation_argument e (use_data_term u) (Payload_Term i)
+      (binding_rows_term [(ib,Target_Term (Whole_Artifact empty_artifact))])
+      (Target_Term (Whole_Artifact empty_artifact))
+      (data_list_term (map Payload_Term Is)) (data_list_term (map Payload_Term Ks)))
+        \<in>positive_meaning scoped_instantiation_system"
+    using interface by (simp_all only: scoped_variable_readings[OF source ib_formed Is(2) Ks(2)])
+  have schema_reads:
+    "(65,schema_instantiation_argument e (use_data_term u) (Payload_Term a)
+      (binding_rows_term [(b,Payload_Term b)]) (Payload_Term b)
+      (call_instance_rows_term [(s,k,package_subject_argument x y z (Payload_Term b))])
+      (binding_rows_term []))\<in>positive_meaning schema_instantiation_system"
+    "(65,schema_instantiation_argument e (use_data_term u) (Payload_Term a)
+      (binding_rows_term [(b,Target_Term (Whole_Artifact empty_artifact))])
+      (Target_Term (Whole_Artifact empty_artifact))
+      (call_instance_rows_term [(s,k,package_subject_argument x y z (Target_Term (Whole_Artifact empty_artifact)))])
+      (binding_rows_term []))\<in>positive_meaning schema_instantiation_system"
+    using origin(4) by (simp_all only: scope_schema_readings[OF source b_formed fields])
+  have rf: "exact_formed R" using ef parts(1) by (auto simp: environment_formed_def)
+  obtain v where presented: "artifact_value_presents R v" using artifact_value_presents_total[OF rf] by blast
+  obtain p q where ports: "ps=[p,q]" using record_at_preserves_socket_occurrences[OF parts(2)]
+    by (auto simp: length_Suc_conv)
+  have admitted: "(72,citation_observation_argument e (use_data_term u) (Payload_Term r) (Payload_Term []))
+      \<in>positive_meaning definition_call_admission_system"
+    by (rule definition_call_admission_complete[OF source raw]) (simp add: octets_formed_def)
+  have lookup: "(37,artifact_lookup_argument e (use_data_term u) v)\<in>positive_meaning artifact_lookup_system"
+    using source parts(1) presented by (auto simp: artifact_lookup_exact)
+  have rec: "(34,rooted_rows_argument v (Payload_Term r)
+      (pair_list_term [(Payload_Term p,Payload_Term i),(Payload_Term q,Payload_Term m)]))
+        \<in>positive_meaning record_admission_system"
+    by (simp only: list.map prod.case record_admission_pair_fields[OF presented]) (use parts(2) ports in auto)
+  have family_read: "(32,rooted_rows_argument v (Payload_Term m)
+      (pair_list_term [(Payload_Term c,Payload_Term a)]))\<in>positive_meaning family_admission_system"
+    using family_admission_rows[OF presented, of m "[(c,a)]"] singleton
+    by (simp add: address_pair_data_def)
+  let ?h="\<lambda>j::nat. if j=0 then e else if j=1 then use_data_term u else if j=2 then Payload_Term r
+    else if j=3 then definition_site_value k else if j=4 then x else if j=5 then y else if j=6 then z
+    else if j=7 then v else if j=8 then Payload_Term p else if j=9 then Payload_Term q
+    else if j=10 then Payload_Term i else if j=11 then Payload_Term m else if j=12 then Payload_Term c
+    else if j=13 then Payload_Term a else if j=14 then Payload_Term ib else if j=15 then Payload_Term b
+    else if j=16 then Payload_Term s else if j=17 then data_list_term (map Payload_Term Is)
+    else data_list_term (map Payload_Term Ks)"
+  show ?thesis by (simp only: scope_forwarding_valuation, rule exI[of _ ?h])
+    (use admitted lookup rec family_read interface_reads schema_reads fields
+      schema_call_formed_target[OF positive_meaning_formed[OF admitted]]
+      schema_call_formed_target[OF positive_meaning_formed[OF lookup]]
+      schema_call_formed_target[OF positive_meaning_formed[OF rec]]
+      schema_call_formed_target[OF positive_meaning_formed[OF family_read]]
+      schema_call_formed_target[OF positive_meaning_formed[OF interface_reads(1)]]
+      schema_call_formed_target[OF positive_meaning_formed[OF schema_reads(1)]]
+      in \<open>auto simp: call_instance_value_def\<close>)
+qed
+
+theorem scope_forwarding_exact:
+  "(116,t)\<in>positive_meaning scope_forwarding_system \<longleftrightarrow> scope_forwarding_result t"
+  using scope_forwarding_sound scope_forwarding_complete by blast
+
+corollary scope_forwarding_on_values:
+  assumes source: "environment_value_presents E e"
+  shows "(116,scope_forwarding_argument e (use_data_term u) (Payload_Term r) (definition_site_value k) x y z)
+    \<in>positive_meaning scope_forwarding_system \<longleftrightarrow> native_scope_forwarding_at E u r k x y z"
+proof -
+  have unique: "F=E" if "environment_value_presents F e" for F
+    by (rule environment_value_presents_unique[OF that source])
+  show ?thesis
+    by (simp only: scope_forwarding_exact factor_term.inject
+        inj_eq[OF use_data_term_injective] definition_site_value_eq)
+      (use source unique in blast)
+qed
+
+corollary scope_forwarding_presentation_invariance:
+  assumes "environment_value_presents E e" "environment_value_presents E f"
+  shows "(116,scope_forwarding_argument e (use_data_term u) (Payload_Term r) (definition_site_value k) x y z)
+      \<in>positive_meaning scope_forwarding_system \<longleftrightarrow>
+    (116,scope_forwarding_argument f (use_data_term u) (Payload_Term r) (definition_site_value k) x y z)
+      \<in>positive_meaning scope_forwarding_system"
+  by (simp only: scope_forwarding_on_values[OF assms(1)] scope_forwarding_on_values[OF assms(2)])
+
+theorem scope_forwarding_admission_total:
+  fixes E :: "local_address option artifact_environment"
+  assumes formed: "environment_formed E"
+    and callee: "\<exists>R. artifact_at E (fst k) R \<and> anchor_formed (R,snd k)"
+    and fields: "term_formed x" "term_formed y" "term_formed z"
+  shows "\<exists>F f u. environment_included E F \<and> u\<notin>environment_uses E \<and>
+    environment_value_presents F f \<and>
+    (116,scope_forwarding_argument f (use_data_term u) (Payload_Term []) (definition_site_value k) x y z)
+      \<in>positive_meaning scope_forwarding_system"
+proof -
+  obtain F u where built: "environment_formed F" "environment_included E F"
+    "u\<notin>environment_uses E" "native_scope_forwarding_at F u [] k x y z"
+    using native_scope_forwarding_total[OF formed callee fields] by blast
+  obtain f where source: "environment_value_presents F f"
+    using environment_value_presents_total[OF built(1)] by blast
+  show ?thesis using built(2,3) source scope_forwarding_complete[OF source built(4)] by blast
+qed
+
+theorem admitted_scope_forwarding_meaning:
+  assumes source: "environment_value_presents E e"
+    and package: "native_package_at E pu pr P" and reference: "native_package_at E qu qr Q"
+    and members: "d\<in>system_definitions P" "k\<in>system_definitions Q"
+    and admitted: "(116,scope_forwarding_argument e (use_data_term (fst d)) (Payload_Term (snd d))
+      (definition_site_value k) x y z)\<in>positive_meaning scope_forwarding_system"
+  shows "schema_call_formed P d w \<longleftrightarrow> term_formed w"
+    and "(d,w)\<in>positive_meaning P \<longleftrightarrow>
+      (k,package_subject_argument x y z w)\<in>positive_meaning Q"
+proof -
+  have read: "native_scope_forwarding_at E (fst d) (snd d) k x y z"
+    using admitted by (simp only: scope_forwarding_on_values[OF source])
+  show "schema_call_formed P d w \<longleftrightarrow> term_formed w"
+    by (rule native_scope_forwarding_call[OF package members(1) read])
+  show "(d,w)\<in>positive_meaning P \<longleftrightarrow>
+      (k,package_subject_argument x y z w)\<in>positive_meaning Q"
+    by (rule native_scope_forwarding_shared_meaning[OF package reference members read])
+qed
+
+section \<open>Complete families exclude omitted alternatives and conditions\<close>
+
+theorem scope_forwarding_empty_clauses_rejected:
+  assumes source: "environment_value_presents E e" and raw: "native_definition_at E u r p {}"
+  shows "(116,scope_forwarding_argument e (use_data_term u) (Payload_Term r) (definition_site_value k) x y z)
+    \<notin>positive_meaning scope_forwarding_system"
+proof
+  assume holds: "(116,scope_forwarding_argument e (use_data_term u) (Payload_Term r) (definition_site_value k) x y z)
+    \<in>positive_meaning scope_forwarding_system"
+  obtain i c b s where read: "native_definition_at E u r (Pattern_Variable i)
+    {(c,scope_call_schema b s k x y z)}"
+    using holds by (simp only: scope_forwarding_on_values[OF source] native_scope_forwarding_at_def) blast
+  have "{}={(c,scope_call_schema b s k x y z)}"
+    using native_definition_unique[OF raw read] by blast
+  then show False by simp
+qed
+
+theorem scope_forwarding_material_clause_rejected:
+  assumes source: "environment_value_presents E e" and raw: "native_definition_at E u r p C"
+    and member: "(c,S)\<in>C" and material: "schema_material_premises S\<noteq>{}"
+  shows "(116,scope_forwarding_argument e (use_data_term u) (Payload_Term r) (definition_site_value k) x y z)
+    \<notin>positive_meaning scope_forwarding_system"
+proof -
+  have rejected: "\<not>native_scope_forwarding_at E u r k x y z"
+  proof
+    assume "native_scope_forwarding_at E u r k x y z"
+    then obtain i d b s where read: "native_definition_at E u r (Pattern_Variable i)
+      {(d,scope_call_schema b s k x y z)}" by (auto simp: native_scope_forwarding_at_def)
+    have "S=scope_call_schema b s k x y z"
+      using native_definition_unique[OF raw read] member by auto
+    then show False using material by (simp add: scope_call_schema_def)
+  qed
+  show ?thesis using rejected by (simp add: scope_forwarding_on_values[OF source])
+qed
+
+theorem scope_forwarding_extra_clause_rejected:
+  assumes source: "environment_value_presents E e" and raw: "native_definition_at E u r p C"
+    and clauses: "(c,S)\<in>C" "(d,T)\<in>C" "c\<noteq>d"
+  shows "(116,scope_forwarding_argument e (use_data_term u) (Payload_Term r) (definition_site_value k) x y z)
+    \<notin>positive_meaning scope_forwarding_system"
+proof
+  assume holds: "(116,scope_forwarding_argument e (use_data_term u) (Payload_Term r) (definition_site_value k) x y z)
+    \<in>positive_meaning scope_forwarding_system"
+  obtain i f b s where read: "native_definition_at E u r (Pattern_Variable i)
+    {(f,scope_call_schema b s k x y z)}"
+    using holds by (simp only: scope_forwarding_on_values[OF source] native_scope_forwarding_at_def) blast
+  have "C={(f,scope_call_schema b s k x y z)}"
+    using native_definition_unique[OF raw read] by blast
+  then show False using clauses by auto
+qed
+
+section \<open>One fixed native checker serves every future submitted definition\<close>
+
+theorem native_scope_forwarding_checker:
+  "\<exists>C :: local_address option artifact_environment. \<exists>cu Q d.
+    closed_native_package_at C cu [] Q \<and>
+    (\<forall>t. term_formed t \<longrightarrow>
+      (\<exists>F au I K. environment_formed F \<and> environment_included C F \<and> au\<notin>environment_uses C \<and>
+        native_package_at F cu [] Q \<and> native_application_at F au [] d t I K \<and>
+        native_package_environment F cu []=C \<and> native_application_formed F cu [] au [] \<and>
+        (native_positive_holds F cu [] au [] \<longleftrightarrow> scope_forwarding_result t) \<and>
+        (\<forall>v\<in>environment_uses C. \<forall>R. artifact_at F v R \<longleftrightarrow> artifact_at C v R) \<and>
+        (\<forall>v\<in>environment_uses C. \<forall>k w. binds_slot F v k w \<longleftrightarrow> binds_slot C v k w)))"
+proof -
+  obtain g :: "nat\<Rightarrow>local_address option definition_site"
+    and C :: "local_address option artifact_environment" and cu Q
+    where closed: "closed_native_package_at C cu [] Q"
+    and future: "\<forall>d\<in>system_definitions scope_forwarding_system. \<forall>t. term_formed t \<longrightarrow>
+      (\<exists>F au I K. environment_formed F \<and> environment_included C F \<and> au\<notin>environment_uses C \<and>
+        native_package_at F cu [] Q \<and> native_application_at F au [] (g d) t I K \<and>
+        native_package_environment F cu []=C \<and>
+        (native_application_formed F cu [] au [] \<longleftrightarrow> schema_call_formed scope_forwarding_system d t) \<and>
+        (native_positive_holds F cu [] au [] \<longleftrightarrow> (d,t)\<in>positive_meaning scope_forwarding_system) \<and>
+        (\<forall>v\<in>environment_uses C. \<forall>R. artifact_at F v R \<longleftrightarrow> artifact_at C v R) \<and>
+        (\<forall>v\<in>environment_uses C. \<forall>k w. binds_slot F v k w \<longleftrightarrow> binds_slot C v k w))"
+    using compiled_program_future_applications[OF scope_forwarding_system_formed] by blast
+  have member: "116\<in>system_definitions scope_forwarding_system" by simp
+  show ?thesis by (rule exI[of _ C], rule exI[of _ cu], rule exI[of _ Q], rule exI[of _ "g 116"])
+    (use closed future[rule_format, OF member] in \<open>auto simp: scope_forwarding_call scope_forwarding_exact\<close>)
+qed
+
+text \<open>
+  Eight ordinary premises inspect the actual definition: native definition
+  admission, source artifact lookup, its complete two-field record, its complete
+  singleton clause family, and two readings each of the interface and schema.
+  Both schema outputs require the complete empty material relation. The finite
+  readings determine syntax; they are not samples of the submitted program's
+  behavior. The callee's actual use and root remain data in those readings.
+
+  In a formed package containing an admitted entry, every formed future argument
+  is accepted and forwarded exactly to its actual callee at the fixed scope.
+  Admission of the definition alone does not supply that package. Shared-package
+  agreement then relates that call to an independently established package.
+  Empty, additional, and material clauses are rejected. Every actual profile
+  and every complete source presentation has admission, and one fixed native
+  checker precedes all future input terms while preserving its original scope.
+
+  This sufficient definition profile does not decide equivalence of arbitrary
+  programs. Historical interpreter admission still has to bind both entries to
+  the actual submitted package and retain a fixed, independently proved
+  interpreter as their common semantic dependency.
+\<close>
+
+end
